more instances; fixes

theories/stacked_borrows/expr_semantics.v
@@ -12,7 +12,7 @@ Fixpoint subst (x : string) (es : expr) (e : expr) : expr :=
   | Val v => Val v
   | Call e1 e2 => Call (subst x es e1) (subst x es e2)
   | InitCall => InitCall
-  | EndCall => EndCall
+  | EndCall e => EndCall (subst x es e)
   | Place l tag T => Place l tag T
   | BinOp op e1 e2 => BinOp op (subst x es e1) (subst x es e2)
   | Proj e1 e2 => Proj (subst x es e1) (subst x es e2)
@@ -80,6 +80,7 @@ Qed.
 Inductive ectx_item :=
 | CallLCtx (r2 : result)
 | CallRCtx (e1 : expr)
+| EndCallCtx
 | BinOpRCtx (op : bin_op) (e1 : expr)
 | BinOpLCtx (op : bin_op) (r2 : result)
 | ProjRCtx (e1 : expr)
@@ -101,6 +102,7 @@ Definition fill_item (Ki : ectx_item) (e : expr) : expr :=
   match Ki with
   | CallLCtx r2 => Call e (of_result r2)
   | CallRCtx e1 => Call e1 e
+  | EndCallCtx => EndCall e
   | BinOpRCtx op e1 => BinOp op e1 e
   | BinOpLCtx op r2 => BinOp op e (of_result r2)
   | ProjRCtx e1 => Proj e1 e
@@ -186,6 +188,7 @@ Inductive scalar_neq : scalar → scalar → Prop :=
 | LocNeqNullL l tag :
     scalar_neq (ScInt 0) (ScPtr l tag).
 
+
 Inductive bin_op_eval h : bin_op → scalar → scalar → scalar → Prop :=
 | BinOpPlus z1 z2 :
     bin_op_eval h AddOp (ScInt z1) (ScInt z2) (ScInt (z1 + z2))
@@ -201,6 +204,28 @@ Inductive bin_op_eval h : bin_op → scalar → scalar → scalar → Prop :=
     scalar_neq l1 l2 → bin_op_eval h EqOp l1 l2 (sc_of_bool false)
 | BinOpOffset l z tag :
     bin_op_eval h OffsetOp (ScPtr l tag) (ScInt z) (ScPtr (l +ₗ z) tag).
+
+Global Hint Constructors scalar_eq : core.
+Global Hint Constructors scalar_neq : core.
+Global Hint Constructors bin_op_eval : core.
+Global Instance scalar_eq_dec h sc1 sc2 : Decision (scalar_eq h sc1 sc2).
+Proof.
+  destruct sc1, sc2; try by (right; intros H; inversion H).
+  - destruct (decide (n = n0)) as [ -> | ]; [left; eauto | right; intros H; inversion H; done].
+  - destruct (decide (l = l0)) as [<- | Hneq]; first by left; eauto.
+    destruct (h !! l) eqn:Heq; last left; eauto.
+    destruct (h !! l0) eqn:Heq'; last left; eauto.
+    right. intros H; inversion H; subst; congruence.
+Qed.
+Global Instance scalar_neq_dec sc1 sc2 : Decision (scalar_neq sc1 sc2).
+Proof.
+  destruct sc1, sc2; try by (right; intros H; inversion H).
+  - destruct (decide (n = n0)) as [-> | Hneq]; [right; intros H; inversion H; congruence | left; eauto].
+  - destruct (decide (n = 0)) as [-> | Hneq]; [left; eauto | right; intros H; inversion H; congruence].
+  - destruct (decide (n = 0)) as [-> | Hneq]; [left; eauto | right; intros H; inversion H; congruence].
+  - destruct (decide (l = l0)) as [<- | Hneq]; [right; intros H; inversion H; congruence | left; eauto].
+Qed.
+
 
 (* Compute subtype of `T` and offset to it from `path` *)
 Fixpoint field_access (T : type) (path : list nat) :
@@ -301,14 +326,17 @@ Inductive pure_expr_step (P : prog) (h : mem) : expr → expr → Prop :=
 (* TODO: initcall should generate a call id explicitly, endcall should take one and end it;
   semantics should have a set of active call_ids.
    ghost state for owning call ids (like heap) -- similar to bijection.
-
-  @LG: should it really? why not just keep following the stack discipline and do not mention the call ids at all in the expr semantics?
 *)
 Inductive mem_expr_step (h: mem) : expr → event → mem → expr → Prop :=
-| InitCallBS :
-    mem_expr_step h InitCall InitCallEvt h #[☠]
-| EndCallBS :
-    mem_expr_step h EndCall EndCallEvt h #[☠]
+  (* TODO: can we remove call_id here?*)
+| InitCallBS (c: call_id):
+    mem_expr_step
+              h InitCall
+              (InitCallEvt c)
+              h (Val(cons (ScCallId c) nil))
+| EndCallBS (call: call_id) e :
+    to_value e = Some [ScCallId call] →
+    mem_expr_step h (EndCall e) (EndCallEvt call) h #[☠]
 | CopyBS l lbor T (v: value)
     (READ: read_mem l (tsize T) h = Some v)
     (* (LEN: length v = tsize T) : true by read_mem_values *)
