theories/stacked_borrows/examples/pure.v
@@ -1,0 +1,19 @@
+From simuliris.stacked_borrows Require Import proofmode.
+
+(** * Some trivial tests to check that the proofmode works *)
+Section boring_lang.
+Context `{sborG Σ}.
+
+Definition val_rel (r1 r2 : result) : iProp Σ := ⌜r1 = r2⌝.
+Local Notation "et '⪯' es {{ Φ }}" := (et ⪯{val_rel} es {{Φ}})%I (at level 40, Φ at level 200) : bi_scope.
+
+Lemma test1 :
+  ⊢ (let: "x" :=  #[ScInt 5] + #[ScInt 5] in "x") ⪯ #[ScInt 10] {{ val_rel }}.
+Proof.
+  (*target_bind (_ + _)%E. *)
+  (*target_bind (Let _ _ _)%E.*)
+  sim_pures.
+  sim_val. eauto.
+Qed.
+
+End boring_lang.
