theories/stacked_borrows/proofmode.v
@@ -2,12 +2,12 @@ From iris.proofmode Require Import coq_tactics reduction.
 From iris.proofmode Require Export tactics.
 From simuliris.simulation Require Import slsls lifting language.
 From simuliris.stacked_borrows Require Import tactics class_instances.
-From simuliris.stacked_borrows Require Export notation primitive_laws.
 From iris.bi Require Import bi.
 Import bi.
 From iris.bi Require Import derived_laws.
 Import bi.
 From iris.prelude Require Import options.
+From simuliris.stacked_borrows Require Export primitive_laws notation.
 
 
 Section sim.
